Refactor type system to use `schema_ty`

Physical.v
@@ -2,19 +2,6 @@ Require Import Pig.Base.
 
 Module Physical.
 
-Inductive ty: Type :=
-| TUnit : ty
-| TFn : ty -> ty -> ty
-| TPred : ty -> ty
-| TNil: ty               (* Schema Tuple Terminator *)
-| TCons: ty -> ty -> ty  (* Schema Tuple Extension Type *)
-| TInt: ty               (* An Atomic Schema Attribute Type *)
-| TBag: ty -> ty.        (* A Compound Schema Attribute Type *)
-
-
-Definition col: Type := nat.
-
-
 Inductive tm: Type :=
  | t_filter: id -> id -> tm
  | t_foreach: id -> id -> tm 
@@ -27,169 +14,35 @@ Inductive tm: Type :=
  | t_seq: tm -> tm -> tm.
 
 
-Inductive schema_ty : ty -> Prop :=
-| STNil:
-    schema_ty TNil
-| STConsInt: forall T,
-    schema_ty T ->
-    schema_ty (TCons TInt T)
-| STConsBag: forall T1 T2,
-    schema_ty T1 ->
-    schema_ty T2 ->
-    schema_ty (TCons (TBag T1) T2).
-
-
-Inductive udf_ty : ty -> Prop := 
-| UDFTFn: forall S1 S2,
-    schema_ty S1 ->
-    schema_ty S2 ->
-    udf_ty (TFn S1 S2)
-| UDFTPred: forall S,
-    schema_ty S ->
-    udf_ty S.
-
-
-Inductive loadable_ty : ty -> Prop :=
-| LTSchema: forall S,
-    schema_ty S ->
-    loadable_ty S
-| LTUDF: forall UDF,
-    udf_ty UDF ->
-    loadable_ty UDF.
-
-
-(* Provides evidence that the given column of a given schema has given type. *)
-Inductive schema_column_has_type: ty -> col -> ty -> Prop :=
-  | SchemaColumnIsIntZero: forall (TSchema T: ty),
-      schema_ty TSchema ->
-      schema_column_has_type TSchema O T
-  | SchemaColumnIsIntSucc: forall (TSchema TSchemaHead TSchemaTail T: ty) c,
-      TSchema = TCons TSchemaHead TSchemaTail ->  (* `THead` is unused. *)
-      schema_ty TSchema ->
-      schema_column_has_type TSchemaTail c T ->
-      schema_column_has_type TSchema (S c) T.
-
-
-(* ################################### *)
-(** *** Typing Relation For Queries *)
-
-(* TODO: Update These! *)
-(**
-
-conventions:
- T : a type
- S : a type which satsifies schema_ty
- x, y: identifiers
- s : a statement
- q : a term of query form
-
-
-                             q = q_id x
-                      Gamma |- x \in TQuery m
-                     -------------------------                 (T_Id)
-                      Gamma |- q \in TQuery m
-
-                        q = q_filter x y
-                             n <= m
-            Gamma |- x \in TQuery m  Gamma |- y \in TPred n
-            -----------------------------------------------    (T_Filter)
-                    Gamma |- q \in TQuery m
-
-                      q = q_foreach x y
-            Gamma |- x \in TQuery m  Gamma |- y \in TFn m n
-            -----------------------------------------------    (T_ForEach)
-                     Gamma |- q \in TQuery n
-
-
-                        q = q_group x y
-                            n <= m
-           Gamma |- x \in TQuery m  Gamma |- y \in TPred n
-           -----------------------------------------------     (T_Group)
-                     Gamma |- q \in TQuery m
-
-                        q = q_join x m y n
-                         m <= m'   n <= n'
-          Gamma |- x \in TQuery m'  Gamma |- y \in TQuery n'
-          -------------------------------------------------    (T_Join)
-                     Gamma |- q \in TQuery (m'+n')
-
-
-(** *** Typing Relation For Statements *)
-
-(**
-
-                            Gamma |- x \in T
-                     --------------------------                (T_Store)
-                     Gamma |- s_store x \in TUnit
-
-                     -----------------------------             (T_Load)
-                     Gamma |- s_load x T \in TUnit
-
-                          s = s_assign x q
-      forall T: Gamma |- x not \in T  Gamma |- q \in TQuery m
-      -------------------------------------------------------  (T_Assign)
-                     Gamma |- s \in TUnit
-
-               s = s_seq s1 s2       s1 = s_load x T
-                     x:T, Gamma |- s2 \in TUnit
-               -------------------------------------           (T_Seq_Load)
-                     Gamma |- s \in TUnit
-
-        s = s_seq s1 s2                 s1 = s_assign x q
-       Gamma |- x \in T              Gamma |- q \in TQuery  
-                   x:T, Gamma |- s2 \in TUnit
-       ---------------------------------------------------     (T_Seq_Assign)
-                     Gamma |- s \in TUnit
-
-                        s = s_seq s1 s2
-         Gamma |- s1 \in TUnit        Gamma |- s2 \in TUnit
-         --------------------------------------------------    (T_Seq)
-                     Gamma |- s \in TUnit
-
-*)
-**)
-
-
-Definition context := partial_map ty.
-
 
 Reserved Notation "Gamma '|-' t '\in' T" (at level 40).
-
 
 Inductive has_type : context -> tm -> ty -> Prop :=
 
   | T_Filter : forall Gamma x y S,
-      Gamma x = Some S ->
+      Gamma x = Some (TSchema S) ->
       Gamma y = Some (TPred S) ->
-      schema_ty S ->
-      Gamma |- t_filter x y \in S
+      Gamma |- t_filter x y \in TSchema S
 
   | T_ForEach : forall Gamma x y S S',
-      Gamma x = Some(S) ->
+      Gamma x = Some(TSchema S) ->
       Gamma y = Some(TFn S S') ->
-      schema_ty S ->
-      schema_ty S' ->
-      Gamma |- t_foreach x y \in S'
+      Gamma |- t_foreach x y \in TSchema S'
 
-  | T_LReArrange : forall Gamma x c S,
-      Gamma x = Some S ->
-      schema_ty S ->
-      schema_column_has_type S c TInt ->
-      Gamma |- t_lrearrange x c \in S
+  | T_LocalRearrange : forall Gamma x c S,
+      Gamma x = Some (TSchema S) ->
+      can_rearrange_by S c ->
+      Gamma |- t_lrearrange x c \in (TSchema S)
 
-  | T_GReArrange : forall Gamma x c S,
-      Gamma x = Some S ->
-      schema_ty S ->
-      schema_column_has_type S c TInt ->
-      Gamma |- t_grearrange x c \in S
+  | T_GlobalRearrange : forall Gamma x c S,
+      Gamma x = Some (TSchema S) ->
+      can_rearrange_by S c ->
+      Gamma |- t_grearrange x c \in (TSchema S)
 
-  | T_Package : forall Gamma x c S S',
-      Gamma x = Some S ->
-      schema_ty S ->
-      schema_ty S' ->
-      schema_column_has_type S c TInt ->
-      S' = TCons TInt (TBag S) ->
-      Gamma |- t_package x c \in S'
+  | T_Package : forall Gamma x c S,
+      Gamma x = Some (TSchema S) ->
+      can_package_by S c ->
+      Gamma |- t_package x c \in TSchema (CTyNat *** (CTyBag S) ***)
 
   | T_Load : forall Gamma x T,
       Gamma x = None ->
@@ -198,13 +51,11 @@ Inductive has_type : context -> tm -> ty -> Prop :=
 
   | T_Assign : forall Gamma x q S,
       Gamma x = None ->
-      Gamma |- q \in S ->
-      schema_ty S ->
+      Gamma |- q \in TSchema S ->
       Gamma |- t_assign x q \in TUnit
 
   | T_Store : forall Gamma x S,
-      Gamma x = Some S ->
-      schema_ty S ->
+      Gamma x = Some (TSchema S) ->
       Gamma |- t_store x \in TUnit
 
   | T_SeqLoad : forall Gamma x T s1 s2,
@@ -215,26 +66,21 @@ Inductive has_type : context -> tm -> ty -> Prop :=
 
   | T_SeqAssign : forall Gamma x q s1 s2 S,
       s1 = t_assign x q ->
-      Gamma |- q \in S ->
-      schema_ty S ->
+      Gamma |- q \in TSchema S ->
       Gamma |- s1 \in TUnit ->
-      extend Gamma x S |- s2 \in TUnit ->
+      extend Gamma x (TSchema S) |- s2 \in TUnit ->
       Gamma |- t_seq s1 s2 \in TUnit
 
   | T_SeqStore : forall Gamma x s1 s2 S,
       s1 = t_store x ->
-      Gamma x = Some S ->
-      schema_ty S ->
+      Gamma x = Some (TSchema S) ->
       Gamma |- s1 \in TUnit ->
       Gamma |- s2 \in TUnit ->
       Gamma |- t_seq s1 s2 \in TUnit
 
-where "Gamma '|-' t '\in' T" := (has_type Gamma t T).
+  where "Gamma '|-' t '\in' T" := (has_type Gamma t T).
 
 Hint Constructors has_type.
-
-
-(* ################################### *)
 
 
 End Physical.
