Logical.v
@@ -1,9 +1,8 @@
-
 Require Export Pig.Base.
 
 Module Logical.
 
-Inductive tm: Type :=
+Inductive tm: Set :=
 | t_filter: id -> id -> tm
 | t_foreach: id -> id -> tm 
 | t_group: id -> col -> tm
@@ -14,126 +13,32 @@ Inductive tm: Type :=
 | t_seq: tm -> tm -> tm.
 
 
-
-
-
-Definition context := partial_map ty.
-
-(* ################################### *)
-(** *** Typing Relation For Queries *)
-
-
-
-(* TODO: Update These! *)
-(**
-
-conventions:
- T : a type
- S : a type which satsifies schema_ty
- x, y: identifiers
- s : a statement
- q : a term of query form
-
-
-                             q = q_id x
-                      Gamma |- x \in TQuery m
-                     -------------------------                 (T_Id)
-                      Gamma |- q \in TQuery m
-
-                        q = q_filter x y
-                             n <= m
-            Gamma |- x \in TQuery m  Gamma |- y \in TPred n
-            -----------------------------------------------    (T_Filter)
-                    Gamma |- q \in TQuery m
-
-                      q = q_foreach x y
-            Gamma |- x \in TQuery m  Gamma |- y \in TFn m n
-            -----------------------------------------------    (T_ForEach)
-                     Gamma |- q \in TQuery n
-
-
-                        q = q_group x y
-                            n <= m
-           Gamma |- x \in TQuery m  Gamma |- y \in TPred n
-           -----------------------------------------------     (T_Group)
-                     Gamma |- q \in TQuery m
-
-                        q = q_join x m y n
-                         m <= m'   n <= n'
-          Gamma |- x \in TQuery m'  Gamma |- y \in TQuery n'
-          -------------------------------------------------    (T_Join)
-                     Gamma |- q \in TQuery (m'+n')
-
-
-(** *** Typing Relation For Statements *)
-
-(**
-
-                            Gamma |- x \in T
-                     --------------------------                (T_Store)
-                     Gamma |- s_store x \in TUnit
-
-                     -----------------------------             (T_Load)
-                     Gamma |- s_load x T \in TUnit
-
-                          s = s_assign x q
-      forall T: Gamma |- x not \in T  Gamma |- q \in TQuery m
-      -------------------------------------------------------  (T_Assign)
-                     Gamma |- s \in TUnit
-
-               s = s_seq s1 s2       s1 = s_load x T
-                     x:T, Gamma |- s2 \in TUnit
-               -------------------------------------           (T_Seq_Load)
-                     Gamma |- s \in TUnit
-
-        s = s_seq s1 s2                 s1 = s_assign x q
-       Gamma |- x \in T              Gamma |- q \in TQuery  
-                   x:T, Gamma |- s2 \in TUnit
-       ---------------------------------------------------     (T_Seq_Assign)
-                     Gamma |- s \in TUnit
-
-                        s = s_seq s1 s2
-         Gamma |- s1 \in TUnit        Gamma |- s2 \in TUnit
-         --------------------------------------------------    (T_Seq)
-                     Gamma |- s \in TUnit
-
-*)
-**)
-
 Reserved Notation "Gamma '|-' t '\in' T" (at level 40).
 
 Inductive has_type : context -> tm -> ty -> Prop :=
 
   | T_Filter : forall Gamma x y S,
-      Gamma x = Some S ->
+      Gamma x = Some (TSchema S) ->
       Gamma y = Some (TPred S) ->
-      schema_ty S ->
-      Gamma |- t_filter x y \in S
+      Gamma |- t_filter x y \in TSchema S
 
   | T_ForEach : forall Gamma x y S S',
-      Gamma x = Some(S) ->
+      Gamma x = Some(TSchema S) ->
       Gamma y = Some(TFn S S') ->
-      schema_ty S ->
-      schema_ty S' ->
-      Gamma |- t_foreach x y \in S'
+      Gamma |- t_foreach x y \in TSchema S'
 
-  | T_Group : forall Gamma x c S S',
-      Gamma x = Some S ->
-      schema_ty S ->
-      schema_ty S' ->
-      schema_column_has_type S c TInt ->
-      S' = TCons TInt (TBag S) ->
-      Gamma |- t_group x c \in S'
+  | T_Group : forall Gamma x c S,
+      Gamma x = Some (TSchema S) ->
+      can_group_by S c ->
+      Gamma |- t_group x c \in TSchema (CTyNat *** (CTyBag S) ***)
 
   | T_Join : forall Gamma x y cx cy S1 S2 S3,
-      Gamma x = Some(S1) ->
-      Gamma y = Some(S2) ->
-      schema_ty S1 ->
-      schema_ty S2 ->
-      schema_column_has_type S1 cx TInt ->
-      schema_column_has_type S2 cy TInt ->
+      Gamma x = Some(TSchema S1) ->
+      Gamma y = Some(TSchema S2) ->
+      can_join_by S1 cx ->
+      can_join_by S2 cy ->
       concatenated_schema S1 S2 S3 ->
-      Gamma |- t_join x cx y cx \in S3
+      Gamma |- t_join x cx y cx \in TSchema S3
 
   | T_Load : forall Gamma x T,
       Gamma x = None ->
@@ -142,13 +47,11 @@ Inductive has_type : context -> tm -> ty -> Prop :=
 
   | T_Assign : forall Gamma x q S,
       Gamma x = None ->
-      Gamma |- q \in S ->
-      schema_ty S ->
+      Gamma |- q \in TSchema S ->
       Gamma |- t_assign x q \in TUnit
 
   | T_Store : forall Gamma x S,
-      Gamma x = Some S ->
-      schema_ty S ->
+      Gamma x = Some (TSchema S) ->
       Gamma |- t_store x \in TUnit
 
   | T_SeqLoad : forall Gamma x T s1 s2,
@@ -159,16 +62,14 @@ Inductive has_type : context -> tm -> ty -> Prop :=
 
   | T_SeqAssign : forall Gamma x q s1 s2 S,
       s1 = t_assign x q ->
-      Gamma |- q \in S ->
-      schema_ty S ->
+      Gamma |- q \in TSchema S ->
       Gamma |- s1 \in TUnit ->
-      extend Gamma x S |- s2 \in TUnit ->
+      extend Gamma x (TSchema S) |- s2 \in TUnit ->
       Gamma |- t_seq s1 s2 \in TUnit
 
   | T_SeqStore : forall Gamma x s1 s2 S,
       s1 = t_store x ->
-      Gamma x = Some S ->
-      schema_ty S ->
+      Gamma x = Some (TSchema S) ->
       Gamma |- s1 \in TUnit ->
       Gamma |- s2 \in TUnit ->
       Gamma |- t_seq s1 s2 \in TUnit
@@ -176,9 +77,5 @@ Inductive has_type : context -> tm -> ty -> Prop :=
 where "Gamma '|-' t '\in' T" := (has_type Gamma t T).
 
 Hint Constructors has_type.
-
-
-(* ################################### *)
-
 
 End Logical.
