Rearranging.v
@@ -1,0 +1,4 @@
+Require Import Pig.Schema.
+
+Definition can_rearrange_by (s: schema_ty) (c: col) : Prop :=
+  schema_column_has_type s c CTyNat.
