Schema.v
@@ -1,0 +1,98 @@
+Require Import SfLib.
+
+
+Inductive schema_ty : Set :=
+  | STyPair: col_ty -> schema_ty -> schema_ty
+  | STyNil: schema_ty
+with col_ty : Set :=
+  | CTyNat: col_ty
+  | CTyBag: schema_ty -> col_ty.
+
+Notation " x *** " := (STyPair x STyNil) (at level 51, right associativity).
+Notation " x '***' y " := (STyPair x y) (at level 51, right associativity).
+
+
+(* Indicates a column within a schema. Used in the JOIN query's BY clauses. *)
+Definition col: Set := nat.
+
+
+(* Provides evidence that the given column of a given schema has given attr. *)
+
+Inductive schema_column_has_type: schema_ty -> col -> col_ty -> Prop :=
+  | SCHAZero: forall (s s': schema_ty) (c: col_ty),
+      s = c *** s' ->
+      schema_column_has_type s O c
+  | SCHASucc: forall (s s': schema_ty) (i i': col) (c c': col_ty),
+      i = S(i') ->
+      s = c' *** s' ->
+      schema_column_has_type s' i c'.
+
+
+Fixpoint schema_concatenation (s1 s2 : schema_ty): schema_ty :=
+  match s1 with
+  | STyNil => s2
+  | c *** => STyPair c s2
+  | c *** s1' => c *** (schema_concatenation s1' s2)
+  end.
+
+
+Inductive concatenated_schema: schema_ty -> schema_ty -> schema_ty -> Prop :=
+| CatSchemaZeroAttr: forall s,
+    concatenated_schema STyNil s s
+| CatSchemaOneAttr: forall a s,
+    concatenated_schema (a ***) s (a *** s)
+| CatSchemaCons: forall a s1 s2 s3,
+    concatenated_schema s1 s2 s3 ->
+    concatenated_schema (a *** s1) s2 (a *** s3).
+
+
+Lemma schema_concatenation_correct: forall (s1 s2: schema_ty),
+  concatenated_schema s1 s2 (schema_concatenation s1 s2).
+Proof.
+  intros. induction s1.
+  - admit.
+  - admit.
+Admitted.
+
+(* The type of each tuple within a relation with the given schema. *)
+Fixpoint support (s: schema_ty) : Type :=
+  match s with
+  | STyNil => unit
+  | a *** => helper a
+  | a *** s' => (helper a) * support s'
+  end
+with helper(c: col_ty) : Type :=
+  match c with
+  | CTyNat => nat
+  | CTyBag s_nested => list (support s_nested)
+  end.
+
+
+Definition relation (s: schema_ty) : Type := list (support s).
+
+
+(* IDEA: Maybe we don't need to model the tuples themselves, just their types.
+         However, we do need to represent sorted lists of tuples, but we can
+         do that using types (see stdlib's `Sorted`). Because of this I am
+         hoping that we don't need to `fuse_tuples`. *)
+
+(*
+Fixpoint fuse_tuples (s1 s2: schema_ty) (t1: support s1) (t2: support s2) :
+                                     support (schema_concatenation s1 s2) := ???
+*)
+
+
+(* An example schema with just one column: a nat column: *)
+Example nat_schema : schema_ty := (CTyNat ***).
+Example nat_tuple : support nat_schema := 1.
+Example nat_relation : relation nat_schema := [1; 2].
+
+(* An example schema with just one column: a bag (of nat): *)
+Example bag_schema := (CTyBag (CTyNat ***) ***).
+Example bag_tuple : support bag_schema := [1; 1].
+Example bag_relation : relation bag_schema := [[1; 2]; [1; 2]].
+
+(* An example schema with two cols: nat and bag of nat. *)
+Example nat_bag_schema : schema_ty := CTyNat *** CTyBag (CTyNat ***) ***.
+Example nat_bag_tuple : support nat_bag_schema := (1, [1; 2; 1]).
+Example nat_bag_relation : relation nat_bag_schema := [(1, [1; 2; 1]); (2, [])].
